LearningLean/Parsing.lean
@@ -1,0 +1,23 @@
+import Mathlib.Logic.Basic
+
+-- An individual parsing error located at a specific span
+def Error := String
+
+-- Any function that can combine multiple inputs of one type into an output of
+-- another type, possibly failing
+def Parser (α β : Type) := α -> Except Error β
+
+-- Matches a specific element, and produces some output after parsing
+def just {α : Type} [BEq α] [ToString α] : α -> Parser α α
+  | a => fun e => if e == a then Except.ok e else Except.error s!"found {e}; expected {a}"
+
+theorem just_matches_x_with_x { α : Type } [BEq α] [ToString α] (x : α) (h : x == x) : just x x = Except.ok x := by
+  unfold just
+  simp [eq_self]
+  exact h
+
+theorem just_does_not_match_a_with_b { α : Type } [BEq α] [LawfulBEq α] [ToString α] (a : α) (b : α) (h : a ≠ b) : just a b = Except.error s!"found {b}; expected {a}" := by
+  unfold just
+  simp [← ne_eq]
+  symm
+  exact h
