lakefile.lean
@@ -1,11 +1,13 @@
 import Lake
 open Lake DSL
 
+require mathlib from git "https://github.com/leanprover-community/mathlib4.git" @ "v4.12.0"
+
 package "learning-lean" where
   -- add package configuration options here
 
 lean_lib «LearningLean» where
-  -- add library configuration options here
+  -- bruh
 
 @[default_target]
 lean_exe "learning-lean" where
